Engine: add direction to bool_tree

Engine/BooleanSemantics.v
@@ -31,88 +31,88 @@ Section BooleanSemantics.
   (** * Boolean Semantics  *)
   (* where checks consult the boolean instead of actually comparing strings *)
 
-  Inductive bool_tree: actions -> input -> LoopBool -> tree -> Prop :=
+  Inductive bool_tree: actions -> input -> LoopBool -> Direction -> tree -> Prop :=
   | tree_done:
     (* nothing to do on an empty list of actions *)
-    forall inp b,
-      bool_tree [] inp b Match
+    forall inp b dir,
+      bool_tree [] inp b dir Match
   | tree_check:
     (* pops a successful check from the action list *)
     (* NEW: this only checks the boolean allows exit and not the strcheck in the tree *)
-    forall inp strcheck cont treecont
-      (TREECONT: bool_tree cont inp CanExit treecont),
-      bool_tree (Acheck strcheck :: cont) inp CanExit (Progress treecont)
+    forall inp strcheck cont treecont dir
+      (TREECONT: bool_tree cont inp CanExit dir treecont),
+      bool_tree (Acheck strcheck :: cont) inp CanExit dir (Progress treecont)
   | tree_check_fail:
   (* pops a failing check from the action list *)
-    forall inp strcheck cont,
-      bool_tree (Acheck strcheck :: cont) inp CannotExit Mismatch
+    forall inp strcheck cont dir,
+      bool_tree (Acheck strcheck :: cont) inp CannotExit dir Mismatch
   | tree_close:
   (* pops the closing of a group from the action list *)
-    forall inp b cont treecont gid
-      (TREECONT: bool_tree cont inp b treecont),
-      bool_tree (Aclose gid :: cont) inp b (GroupAction (Close gid) treecont)
+    forall inp b cont treecont gid dir
+      (TREECONT: bool_tree cont inp b dir treecont),
+      bool_tree (Aclose gid :: cont) inp b dir (GroupAction (Close gid) treecont)
   | tree_epsilon:
-    forall inp b cont tcont
-      (ISTREE: bool_tree cont inp b tcont),
-      bool_tree ((Areg Epsilon)::cont) inp b tcont
+    forall inp b cont tcont dir
+      (ISTREE: bool_tree cont inp b dir tcont),
+      bool_tree ((Areg Epsilon)::cont) inp b dir tcont
   | tree_char:
-    forall c cd inp b nextinp cont tcont
-      (READ: read_char rer cd inp forward = Some (c, nextinp))
+    forall c cd inp b nextinp cont tcont dir
+      (READ: read_char rer cd inp dir = Some (c, nextinp))
       (* NEW: changes the boolean to CanExit *)
-      (TREECONT: bool_tree cont nextinp CanExit tcont),
-      bool_tree (Areg (Regex.Character cd) :: cont) inp b (Read c tcont)
+      (TREECONT: bool_tree cont nextinp CanExit dir tcont),
+      bool_tree (Areg (Regex.Character cd) :: cont) inp b dir (Read c tcont)
   | tree_char_fail:
-    forall cd inp b cont
-      (READ: read_char rer cd inp forward = None),
-      bool_tree (Areg (Regex.Character cd) :: cont) inp b Mismatch
+    forall cd inp b cont dir
+      (READ: read_char rer cd inp dir = None),
+      bool_tree (Areg (Regex.Character cd) :: cont) inp b dir Mismatch
   | tree_disj:
-    forall r1 r2 cont t1 t2 inp b
-      (ISTREE1: bool_tree (Areg r1 :: cont) inp b t1)
-      (ISTREE2: bool_tree (Areg r2 :: cont) inp b t2),
-      bool_tree (Areg (Disjunction r1 r2) :: cont) inp b (Choice t1 t2)
+    forall r1 r2 cont t1 t2 inp b dir
+      (ISTREE1: bool_tree (Areg r1 :: cont) inp b dir t1)
+      (ISTREE2: bool_tree (Areg r2 :: cont) inp b dir t2),
+      bool_tree (Areg (Disjunction r1 r2) :: cont) inp b dir (Choice t1 t2)
   | tree_sequence:
     (* adding next regex to the continuation *)
-    forall r1 r2 cont t inp b
-      (CONT: bool_tree (Areg r1 :: Areg r2 :: cont) inp b t),
-      bool_tree (Areg (Sequence r1 r2) :: cont) inp b t
+    forall r1 r2 cont t inp b dir
+      (CONT: bool_tree (seq_list r1 r2 dir ++ cont) inp b dir t),
+      bool_tree (Areg (Sequence r1 r2) :: cont) inp b dir t
   | tree_quant_forced:
     (* the quantifier is forced to iterate, because there is a strictly positive minimum *)
-    forall r1 greedy min plus cont titer inp b gidl
+    forall r1 greedy min plus cont titer inp b gidl dir
       (* the list of capture groups to reset *)
       (RESET: gidl = def_groups r1)
       (* doing one iteration *)
-      (ISTREE1: bool_tree (Areg r1 :: Areg (Quantified greedy min plus r1) :: cont) inp b titer),
-      bool_tree (Areg (Quantified greedy (S min) plus r1) :: cont) inp b (GroupAction (Reset gidl) titer)
+      (ISTREE1: bool_tree (Areg r1 :: Areg (Quantified greedy min plus r1) :: cont) inp b dir titer),
+      bool_tree (Areg (Quantified greedy (S min) plus r1) :: cont) inp b dir (GroupAction (Reset gidl) titer)
   | tree_quant_done:
     (* the quantifier is done iterating, because min and max are zero *)
-    forall r1 greedy cont tskip inp b
-      (SKIP: bool_tree cont inp b tskip),
-      bool_tree (Areg (Quantified greedy 0 (NoI.N 0) r1) :: cont) inp b tskip
+    forall r1 greedy cont tskip inp b dir
+      (SKIP: bool_tree cont inp b dir tskip),
+      bool_tree (Areg (Quantified greedy 0 (NoI.N 0) r1) :: cont) inp b dir tskip
   | tree_quant_free:
     (* the quantifier is free to iterate or stop *)
-    forall r1 greedy plus cont titer tskip tquant inp b gidl
+    forall r1 greedy plus cont titer tskip tquant inp b gidl dir
       (* the list of capture groups to reset *)
       (RESET: gidl = def_groups r1)
       (* doing one iteration, then a check, then executing the next quantifier *)
       (* NEW: switching the boolean to CannotExit *)
-      (ISTREE1: bool_tree (Areg r1 :: Acheck inp :: Areg (Quantified greedy 0 plus r1) :: cont) inp CannotExit titer)
+      (ISTREE1: bool_tree (Areg r1 :: Acheck inp :: Areg (Quantified greedy 0 plus r1) :: cont) inp CannotExit dir titer)
       (* skipping the quantifier entirely *)
-      (SKIP: bool_tree cont inp b tskip)
+      (SKIP: bool_tree cont inp b dir tskip)
       (CHOICE: tquant = greedy_choice greedy (GroupAction (Reset gidl) titer) tskip),
-      bool_tree (Areg (Quantified greedy 0 (NoI.N 1 + plus)%NoI r1) :: cont) inp b tquant
+      bool_tree (Areg (Quantified greedy 0 (NoI.N 1 + plus)%NoI r1) :: cont) inp b dir tquant
   | tree_group:
-    forall r1 cont treecont inp b gid
-      (TREECONT: bool_tree (Areg r1 :: Aclose gid :: cont) inp b treecont),
-      bool_tree (Areg (Group gid r1) :: cont) inp b (GroupAction (Open gid) treecont)
+    forall r1 cont treecont inp b gid dir
+      (TREECONT: bool_tree (Areg r1 :: Aclose gid :: cont) inp b dir treecont),
+      bool_tree (Areg (Group gid r1) :: cont) inp b dir (GroupAction (Open gid) treecont)
   | tree_anchor:
-    forall a cont treecont inp b
+    forall a cont treecont inp b dir
       (ANCHOR: anchor_satisfied rer a inp = true)
-      (TREECONT: bool_tree cont inp b treecont),
-      bool_tree (Areg (Anchor a) :: cont) inp b (AnchorPass a treecont)
+      (TREECONT: bool_tree cont inp b dir treecont),
+      bool_tree (Areg (Anchor a) :: cont) inp b dir (AnchorPass a treecont)
   | tree_anchor_fail:
-    forall a cont inp b
+    forall a cont inp b dir
       (ANCHOR: anchor_satisfied rer a inp = false),
-      bool_tree (Areg (Anchor a) :: cont) inp b Mismatch.
+      bool_tree (Areg (Anchor a) :: cont) inp b dir Mismatch.
 
 
 (** * Boolean Tree Equivalence  *)
@@ -124,45 +124,66 @@ Section BooleanSemantics.
 
 (** * First Step: encoding the invariant  *)
 
-Inductive bool_encoding: LoopBool -> input -> actions -> Prop :=
+Inductive bool_encoding: LoopBool -> input -> actions -> Direction -> Prop :=
 (* an empty continuation can be encoded with any boolean *)
 | nil_encode:
-  forall str b,
-    bool_encoding b str []
+  forall str b dir,
+    bool_encoding b str [] dir
 | cons_reg:
-  forall b str cont r
-    (ENCODE: bool_encoding b str cont),
-    bool_encoding b str (Areg r::cont)
+  forall b str cont r dir
+    (ENCODE: bool_encoding b str cont dir),
+    bool_encoding b str (Areg r::cont) dir
 | cons_close:
-  forall b str cont gid
-    (ENCODE: bool_encoding b str cont),
-    bool_encoding b str (Aclose gid::cont)
+  forall b str cont gid dir
+    (ENCODE: bool_encoding b str cont dir),
+    bool_encoding b str (Aclose gid::cont) dir
 | cons_true:
-  forall stk str head
-    (ENCODE: bool_encoding CanExit str stk)
-    (STRICT: strict_suffix str head forward),
-    bool_encoding CanExit str (Acheck head::stk)
+  forall stk str head dir
+    (ENCODE: bool_encoding CanExit str stk dir)
+    (STRICT: strict_suffix str head dir),
+    bool_encoding CanExit str (Acheck head::stk) dir
 | cons_false:
   (* when we push the current string to the stack *)
-  forall b stk str
-    (ENCODE: bool_encoding b str stk),
-    bool_encoding CannotExit str (Acheck str::stk).
+  forall b stk str dir
+    (ENCODE: bool_encoding b str stk dir),
+    bool_encoding CannotExit str (Acheck str::stk) dir.
 
 
 (* when we are already encoded with true, reading a new character preserves this true encoding *)
 (* when we are encoded with false, reading a new character switches to being encoded with true *)
-Lemma true_encoding:
+Lemma true_encoding_forward:
   forall str c pref cont b,
-    bool_encoding b (Input (c::str) pref) cont ->
-    bool_encoding CanExit (Input str (c::pref)) cont.
+    bool_encoding b (Input (c::str) pref) cont forward ->
+    bool_encoding CanExit (Input str (c::pref)) cont forward.
 Proof.
   intros str c pref cont b H.
   remember (Input (c::str) pref) as prevstr.
-  induction H; intros.
+  remember forward as dir.
+  induction H; intros; subst.
   - constructor.
   - constructor; auto.
   - constructor; auto.
-  - constructor; auto. rewrite Heqprevstr in STRICT.
+  - constructor; auto.
+    eapply ss_next; eauto. simpl. auto.
+  - constructor.
+    + apply IHbool_encoding; auto.
+    + subst. simpl.
+      eapply ss_advance; eauto.
+Qed.
+
+Lemma true_encoding_backward:
+  forall str c next cont b,
+    bool_encoding b (Input next (c::str)) cont backward ->
+    bool_encoding CanExit (Input (c::next) str) cont backward.
+Proof.
+  intros str c next cont b H.
+  remember (Input next (c::str)) as nextstr.
+  remember backward as dir.
+  induction H; intros; subst.
+  - constructor.
+  - constructor; auto.
+  - constructor; auto.
+  - constructor; auto.
     eapply ss_next; eauto. simpl. auto.
   - constructor.
     + apply IHbool_encoding; auto.
@@ -172,12 +193,12 @@ Qed.
 
 (* if the string is different than the check, we know the boolean is true *)
 Lemma encoding_different:
-  forall b str strcheck cont,
-    bool_encoding b str (Acheck strcheck::cont) ->
+  forall b str strcheck cont dir,
+    bool_encoding b str (Acheck strcheck::cont) dir ->
     str <> strcheck ->
     b = CanExit.
 Proof.
-  intros b0 str [strcheck pref] cont H.
+  intros b0 str [strcheck pref] cont dir H.
   remember (Acheck (Input strcheck pref)::cont) as prevcont.
   induction H; intros; auto; inversion Heqprevcont;
     exfalso; auto.
@@ -185,32 +206,32 @@ Qed.
 
 (* if the check is going to fail, we know the boolean is false *)
 Lemma encoding_same:
-  forall b str cont,
-    bool_encoding b str (Acheck str::cont) -> b = CannotExit.
+  forall b str cont dir,
+    bool_encoding b str (Acheck str::cont) dir -> b = CannotExit.
 Proof.
-  intros b str cont H.
+  intros b str cont dir H.
   remember (Acheck str::cont) as prevcont.
   induction H; intros; auto; inversion Heqprevcont.
   subst. apply ss_neq in STRICT. contradiction.
 Qed.
 
 Lemma encode_next:
-  forall b inp cont r,
-    bool_encoding b inp (Areg r::cont) <->
-    bool_encoding b inp cont.
+  forall b inp cont r dir,
+    bool_encoding b inp (Areg r::cont) dir <->
+    bool_encoding b inp cont dir.
 Proof.
-  intros b inp cont r. split; intros H.
+  intros b inp cont r dir. split; intros H.
   - inversion H; subst.
     inversion ENCODE; subst; auto.
   - destruct inp. constructor. inversion H; subst; auto.
 Qed.
 
 Lemma encode_close:
-  forall b inp cont g,
-    bool_encoding b inp (Aclose g::cont) <->
-    bool_encoding b inp cont.
+  forall b inp cont g dir,
+    bool_encoding b inp (Aclose g::cont) dir <->
+    bool_encoding b inp cont dir.
 Proof.
-  intros b inp cont g. split; intros H.
+  intros b inp cont g dir. split; intros H.
   - inversion H; subst.
     inversion ENCODE; subst; auto.
   - destruct inp. constructor. inversion H; subst; auto.
@@ -220,10 +241,10 @@ Qed.
 (* Here we encode the invariant that the current input is always either equal or strict suffix of any checks in the current list of actions *)
 
 Lemma encoding_suffix:
-  forall b inp act chk,
-    bool_encoding b inp act ->
+  forall b inp act chk dir,
+    bool_encoding b inp act dir ->
     In (Acheck chk) act ->
-    inp = chk \/ strict_suffix inp chk forward.
+    inp = chk \/ strict_suffix inp chk dir.
 Proof.
   intros. induction H.
   - inversion H0.
@@ -239,23 +260,22 @@ Qed.
 (* the two tree constructions are equal *)
 
 Theorem encode_equal:
-  forall inp cont b t gm
+  forall inp cont b dir t gm
     (PIKE: pike_actions cont)
-    (ENCODE: bool_encoding b inp cont)
-    (TREE: is_tree rer cont inp gm forward t),
-    bool_tree cont inp b t.
+    (ENCODE: bool_encoding b inp cont dir)
+    (TREE: is_tree rer cont inp gm dir t),
+    bool_tree cont inp b dir t.
 Proof.
-  intros inp cont b t gm PIKE ENCODE TREE.
+  intros inp cont b dir t gm PIKE ENCODE TREE.
   generalize dependent b.
-  remember forward as dir.
   induction TREE; inversion PIKE; subst; intros;
-    try solve[constructor; auto]; try solve [inversion H1; inversion H0].
+    try solve[constructor; auto]; try solve[inversion H1; inversion H0].
   - assert (b = CanExit).
     { eapply encoding_different; eauto.
       eapply ss_neq; eauto. }
     subst. constructor. eapply IHTREE; eauto.
     inversion ENCODE; subst; auto.
-  - assert (inp = strcheck \/ strict_suffix inp strcheck forward).
+  - assert (inp = strcheck \/ strict_suffix inp strcheck dir).
     { eapply encoding_suffix; eauto. simpl. auto. }
     destruct H; try contradiction. subst.
     assert (b = CannotExit).
@@ -268,8 +288,11 @@ Proof.
   - apply encode_next in ENCODE.
     subst. econstructor; eauto. apply IHTREE; auto.
     destruct nextinp. destruct inp. simpl in READ.
-    destruct next0; inversion READ. destruct (char_match rer t cd); inversion READ; subst.
-    eapply true_encoding; eauto.
+    destruct dir.
+    + destruct next0; inversion READ. destruct (char_match rer t cd); inversion READ; subst.
+      eapply true_encoding_forward; eauto.
+    + destruct pref0; inversion READ. destruct (char_match rer t cd); inversion READ; subst.
+      eapply true_encoding_backward; eauto.
   - apply encode_next in ENCODE. inversion H1. inversion H0. subst. constructor.
     + apply IHTREE1; auto.
       { pike_subset. }
@@ -277,9 +300,9 @@ Proof.
     + apply IHTREE2; auto.
       { pike_subset. }
       apply encode_next. auto.
-  - constructor. subst. simpl in IHTREE. apply IHTREE; eauto.
-    { pike_subset. }
-    inversion ENCODE; subst; constructor; constructor; auto.
+  - constructor. apply IHTREE; eauto.
+    { destruct dir; pike_subset. }
+    destruct dir; inversion ENCODE; subst; constructor; constructor; auto.
   - inversion ENCODE. subst. constructor; auto.
   - destruct (destruct_delta (NoI.N 1 + plus)%NoI) as [DZ | [D1 | [DINF | [delta' [DUN N3]]]]].
     (* Zero repetitions *)
@@ -313,12 +336,12 @@ Proof.
 Qed.
 
 Corollary boolean_correct:
-  forall r inp t,
+  forall r inp dir t,
     pike_regex r ->
-    is_tree rer [Areg r] inp GroupMap.empty forward t ->
-    bool_tree [Areg r] inp CanExit t.
+    is_tree rer [Areg r] inp GroupMap.empty dir t ->
+    bool_tree [Areg r] inp CanExit dir t.
 Proof.
-  intros r str t PIKE H.
+  intros r str dir t PIKE H.
   eapply encode_equal; eauto.
   { constructor; constructor; auto. }
   constructor. constructor.
@@ -327,15 +350,17 @@ Qed.
 
 (* Pike actions translate to Pike trees *)
 Theorem subset_semantics:
-  forall actions tree inp b
+  forall actions tree inp b dir
     (SUBSET: pike_actions actions)
-    (ISTREE: bool_tree actions inp b tree),
+    (ISTREE: bool_tree actions inp b dir tree),
     pike_subtree tree.
 Proof.
-  intros actions tree inp b SUBSET ISTREE.
-  induction ISTREE; try eapply IHISTREE; pike_subset.
-  - eapply IHISTREE1. pike_subset.
-  - eapply IHISTREE2. pike_subset.
+  intros actions tree inp b dir SUBSET ISTREE.
+  induction ISTREE;
+    pike_subset;
+    try (eapply IHISTREE || eapply IHISTREE1 || eapply IHISTREE2);
+    pike_subset.
+  - destruct dir; pike_subset.
   - destruct plus; inversion H3. destruct greedy; pike_subset.
     + eapply IHISTREE1. pike_subset.
     + eapply IHISTREE1. pike_subset.
@@ -344,19 +369,18 @@ Proof.
     + eapply IHISTREE1. pike_subset.
     + eapply IHISTREE1. pike_subset.
   - destruct plus; inversion H3.
-  - eapply IHISTREE. pike_subset.
 Qed.
 
 (** * Determinism  *)
 (* I can't use determinism of is_tree since I've only proved one direction of equivalence *)
 
   Theorem bool_tree_determ:
-    forall actions i b t1 t2,
-      bool_tree actions i b t1 ->
-      bool_tree actions i b t2 ->
+    forall actions i b dir t1 t2,
+      bool_tree actions i b dir t1 ->
+      bool_tree actions i b dir t2 ->
       t1 = t2.
   Proof.
-    intros actions i b t1 t2 H H0.
+    intros actions i b dir t1 t2 H H0.
     generalize dependent t2.
     induction H; intros;
       try solve[inversion H0; subst; auto; f_equal; apply IHbool_tree; auto].
@@ -382,16 +406,16 @@ Qed.
 (* the other direction of implication is obtained using only determinism and productivity *)
 
   Theorem bool_to_istree:
-    forall acts b inp t,
-      bool_encoding b inp acts ->
+    forall acts b inp dir t,
+      bool_encoding b inp acts dir ->
       pike_actions acts ->
-      bool_tree acts inp b t ->
-      is_tree rer acts inp GroupMap.empty forward t.
+      bool_tree acts inp b dir t ->
+      is_tree rer acts inp GroupMap.empty dir t.
   Proof.
-    intros acts b inp t ENCODE H H0.
+    intros acts b inp dir t ENCODE H H0.
     (* productivity *)
-    assert (exists t', is_tree rer acts inp GroupMap.empty forward t') as [t' ISTREE].
-    { destruct (compute_tree rer acts inp  GroupMap.empty forward (S (actions_fuel acts inp forward))) eqn:PROD.
+    assert (exists t', is_tree rer acts inp GroupMap.empty dir t') as [t' ISTREE].
+    { destruct (compute_tree rer acts inp  GroupMap.empty dir (S (actions_fuel acts inp dir))) eqn:PROD.
       2: { generalize functional_terminates. intros H1. apply H1 in PROD; auto; lia. }
       exists t0. eapply compute_is_tree; eauto. }
     eapply encode_equal in ISTREE as BOOLTREE; eauto.
@@ -400,24 +424,24 @@ Qed.
   Qed.
 
   Theorem bool_to_istree_regex:
-    forall r inp t,
+    forall r inp dir t,
       pike_regex r ->
-      bool_tree [Areg r] inp CanExit t ->
-      is_tree rer [Areg r] inp GroupMap.empty forward t.
+      bool_tree [Areg r] inp CanExit dir t ->
+      is_tree rer [Areg r] inp GroupMap.empty dir t.
   Proof.
-    intros r inp t H H0.
-    assert (bool_encoding CanExit inp [Areg r]) by (constructor; constructor).
+    intros r inp dir t H H0.
+    assert (bool_encoding CanExit inp [Areg r] dir) by (constructor; constructor).
     eapply bool_to_istree; eauto; pike_subset.
   Qed.
 
 
   Theorem booltree_istree_equiv:
-    forall r inp t,
+    forall r inp dir t,
       pike_regex r ->
-      bool_tree [Areg r] inp CanExit t <->
-      is_tree rer [Areg r] inp GroupMap.empty forward t.
+      bool_tree [Areg r] inp CanExit dir t <->
+      is_tree rer [Areg r] inp GroupMap.empty dir t.
   Proof.
-    intros r inp t SUBSET. split.
+    intros r inp dir t SUBSET. split.
     - apply bool_to_istree_regex; auto.
     - apply boolean_correct; auto.
   Qed.
